src/Disk/Sectors.v
@@ -1,4 +1,4 @@
-Require Import Bytes.
+Require Import Helpers.
 Require Import Omega.
 
 (* Very basic definitions for modeling disks. *)
